precision.v
@@ -12,53 +12,6 @@ Require Import LIR.dyn.
 
 
 
-(*
-τ ⊑ ★
-
-int ⊑ int
-
-σ₁ ⊑ σ₂    τ₁ ⊑ τ₂
------------------------
-fun[σ₁→τ₁] ⊑ fun[σ₂→τ₂]
-
-Lemma. ⊑ is reflexive and transitive.
-
-Precision on terms of LIR.
-
-Environments Γ⊑ ::= ∅ | Γ⊑, x : σ ⊑ τ
-
-| ∅ |ₗ              =  ∅
-| Γ⊑, x : σ ⊑ τ |ₗ  =  | Γ⊑ |ₗ, x : σ
-
-| ∅ |ᵣ              =  ∅
-| Γ⊑, x : σ ⊑ τ |ᵣ  =  | Γ⊑ |ᵣ, x : τ
-
-| ∅ ∣ₗᵣ             =  ∅
-| Γ, x : τ |ₗᵣ      =  | Γ |ₗᵣ, x : τ ⊑ τ 
-
-The general relation is of the form Γ⊑ ⊢ d ⊑ e : σ ⊑ τ.
-
-Lemma. If Γ⊑ ⊢ d ⊑ e : σ ⊑ τ then σ ⊑ τ and | Γ⊑ |ₗ ⊢ d : σ and | Γ⊑ |ᵣ ⊢ e : τ.
-
-Γ⊑ ⊢ d ⊑ e : ★ ⊑ ★
-----------------------------------    ???
-Γ⊑ ⊢ box[g](d) ⊑ box[g](e) : g ⊑ g
-
-Γ⊑ ⊢ d ⊑ e : ★ ⊑ ★
-----------------------------
-Γ⊑ ⊢ unbox[g](d) ⊑ e : g ⊑ ★
-
-Γ⊑ ⊢ d ⊑ e : g ⊑ ★
-----------------------------
-Γ⊑ ⊢ d ⊑ unbox[g](e) : g ⊑ g
-
-Γ⊑ ⊢ d ⊑ e : g ⊑ ★
---------------------------
-Γ⊑ ⊢ box[g](d) ⊑ e : ★ ⊑ ★
-
-*)
-
-
 Reserved Infix "<|" (at level 80).
 
 
@@ -85,24 +38,34 @@ Proof.
   induction H12; intros ? H23; auto using TPrecision;
   inversion H23; subst; auto using TPrecision.
 Qed.
-  
 
-Inductive PEnvEntry : Type :=
-| pent : forall t1 t2, t1 <| t2 -> PEnvEntry
-.
 
-Definition PEnvironment := Map PEnvEntry.
+Lemma TPFun : forall t1 t2, IRTFun t1 t2 <| Tag2Type TgFun.
+Proof.
+  intros t1 t2.
+  simpl. auto using TPrecision.
+Qed.
+
+
+Lemma GroundFlat: forall g g', (Tag2Type g) <| (Tag2Type g') -> g = g'.
+Proof.
+  intros g g'.
+  destruct g; destruct g'; easy.
+Qed.
+
+
+Definition PEnvironment := Map (IRType * IRType).
 
 
 Fixpoint PEnv1 (Γ : PEnvironment) : IREnvironment :=
   match Γ with
   | MEmpty => MEmpty
-  | MCons k (pent t _ _) Γ' => MCons k t (PEnv1 Γ')
+  | MCons var (t, _) Γ' => MCons var t (PEnv1 Γ')
   end.
 
 
-Lemma InP1 : forall Γ var t1 t2 p,
-    In Γ var = Some (pent t1 t2 p) -> In (PEnv1 Γ) var = Some t1.
+Lemma InP1 : forall Γ var t1 t2,
+    In Γ var = Some (t1, t2) -> In (PEnv1 Γ) var = Some t1.
 Proof.
   intros Γ var t1 t2 HIn.
   induction Γ.
@@ -115,12 +78,12 @@ Qed.
 Fixpoint PEnv2 (Γ : PEnvironment) : IREnvironment :=
   match Γ with
   | MEmpty => MEmpty
-  | MCons k (pent _ t _) Γ' => MCons k t (PEnv2 Γ')
+  | MCons var (_, t) Γ' => MCons var t (PEnv2 Γ')
   end.
 
 
-Lemma InP2 : forall Γ var t1 t2 p,
-    In Γ var = Some (pent t1 t2 p) -> In (PEnv2 Γ) var = Some t2.
+Lemma InP2 : forall Γ var t1 t2,
+    In Γ var = Some (t1,  t2) -> In (PEnv2 Γ) var = Some t2.
 Proof.
   intros Γ var t1 t2 HIn.
   induction Γ.
@@ -133,7 +96,7 @@ Qed.
 Fixpoint Env2P (Γ : IREnvironment) : PEnvironment :=
   match Γ with
   | MEmpty => MEmpty
-  | MCons k t Γ' => MCons k (pent t t (TPrecisionRefl t)) (Env2P Γ')
+  | MCons var t Γ' => MCons var (t,  t) (Env2P Γ')
   end.
 
 
@@ -146,7 +109,7 @@ Qed.
 
 Lemma InP12 : forall Γ var t,
     In Γ var = Some t ->
-    In (Env2P Γ) var = Some (pent t t (TPrecisionRefl t)).
+    In (Env2P Γ) var = Some (t, t).
 Proof.
   intros Γ var t HIn.
   induction Γ.
@@ -157,10 +120,10 @@ Proof.
 Qed.
 
 
-Lemma InE2PType : forall Γ var t1 t2 p,
-  In (Env2P Γ) var = Some (pent t1 t2 p) -> t1 = t2.
+Lemma InE2PType : forall Γ var t1 t2,
+  In (Env2P Γ) var = Some (t1, t2) -> t1 = t2.
 Proof.
-  intros Γ var t1 t2 p HIn.
+  intros Γ var t1 t2 HIn.
   induction Γ.
   - discriminate.
   - simpl in *; breakStrDec; auto;
@@ -168,15 +131,19 @@ Proof.
 Qed.
 
 
-Lemma InE2PVar : forall Γ var t1 t2 p,
-  In (Env2P Γ) var = Some (pent t1 t2 p) -> In Γ var = Some t2.
+Lemma InE2PVar : forall Γ var t1 t2,
+  In (Env2P Γ) var = Some (t1, t2) -> In Γ var = Some t2.
 Proof.
-  intros Γ var t1 t2 p HIn.
+  intros Γ var t1 t2 HIn.
   induction Γ.
   - discriminate.
   - simpl in *; breakStrDec; auto;
     injection HIn; intros; subst; trivial.
 Qed.
+
+
+Definition PEnvP (Γ : PEnvironment) : Prop :=
+  forall var t1 t2, In Γ var = Some (t1, t2) -> t1 <| t2.
 
 
 Inductive Precision : PEnvironment -> IRE -> IRType ->
@@ -187,8 +154,8 @@ Inductive Precision : PEnvironment -> IRE -> IRType ->
 (* Γ⊑ ∋ (x : σ ⊑ τ)
 ------------------
 Γ⊑ ⊢ x ⊑ x : σ ⊑ τ	*)
-| PVar : forall Γ var t1 t2 p,
-    In Γ var = Some (pent t1 t2 p) ->
+| PVar : forall Γ var t1 t2,
+    In Γ var = Some (t1,  t2) ->
     Precision Γ (IREVar var) t1 (IREVar var) t2
 
 (* ----------------------
@@ -229,8 +196,9 @@ Inductive Precision : PEnvironment -> IRE -> IRType ->
 (* Γ⊑, x : σ ⊑ τ ⊢ d ⊑ e : σ′ ⊑ τ′
    ------------------------------------------------
    Γ⊑ ⊢ (λx:σ.d) ⊑ (λx:τ.e) : fun[σ→σ′] ⊑ fun[τ→τ′]	*)
-| PFun : forall Γ var t1 t2 lt12 d1 t1' d2 t2',
-    Precision (var |=> pent t1 t2 lt12; Γ) d1 t1' d2 t2' ->
+| PFun : forall Γ var t1 t2 d1 t1' d2 t2',
+    t1 <| t2 ->
+    Precision (var |=> (t1,  t2); Γ) d1 t1' d2 t2' ->
     Precision Γ (IREFun var t1 d1) (IRTFun t1 t1')
                 (IREFun var t2 d2) (IRTFun t2 t2')
 
@@ -242,49 +210,67 @@ Inductive Precision : PEnvironment -> IRE -> IRType ->
     Precision Γ v1 t1 v2 t2 ->
     Precision Γ (IREFunApp f1 v1) t1' (IREFunApp f2 v2) t2'
 
-(* Γ⊑ ⊢ d ⊑ e : g ⊑ g
-   ----------------------------------
-   Γ⊑ ⊢ box[g](d) ⊑ box[g](e) : ★ ⊑ ★	*)
-| PBox : forall Γ d e g,
-    Precision Γ d (Tag2Type g) e (Tag2Type g) ->
-    Precision Γ (IREBox g d) IRTStar (IREBox g e) IRTStar
-
-(* Γ⊑ ⊢ d ⊑ e : g ⊑ g
+(* Γ⊑ ⊢ d ⊑ e : t ⊑ g
    ----------------------------------
    Γ⊑ ⊢ d ⊑ box[g](e) : g ⊑ ★	*)
-| PBoxR : forall Γ d e g,
-    Precision Γ d (Tag2Type g) e (Tag2Type g) ->
-    Precision Γ d (Tag2Type g) (IREBox g e) IRTStar
+| PBoxR : forall Γ d e t g,
+    Precision Γ d t e (Tag2Type g) ->
+    Precision Γ d t (IREBox g e) IRTStar
+
+(* Γ⊑ ⊢ d ⊑ e : g ⊑ ★
+   ----------------------------------
+   Γ⊑ ⊢ box[g]d ⊑ e : ★ ⊑ ★	*)
+| PBoxL : forall Γ d e g,
+    Precision Γ d (Tag2Type g) e IRTStar ->
+    Precision Γ (IREBox g d) IRTStar e IRTStar
 
 (* Γ⊑ ⊢ d ⊑ e : ★ ⊑ ★
    ----------------------------------
-   Γ⊑ ⊢ unbox[g](d) ⊑ unbox[g](e) : g ⊑ g	*)
-| PUnbox : forall Γ d e g,
-    Precision Γ d IRTStar e IRTStar ->
-    Precision Γ (IREUnbox g d) (Tag2Type g) (IREUnbox g e) (Tag2Type g)
-
-(* Γ⊑ ⊢ d ⊑ e : ★ ⊑ ★
-   ----------------------------------
-   Γ⊑ ⊢ unbox[g](d) ⊑ e : g ⊑ *	*)
+   Γ⊑ ⊢ unbox[g](d) ⊑ e : g ⊑ *		*)
 | PUnboxL : forall Γ d e g,
     Precision Γ d IRTStar e IRTStar ->
     Precision Γ (IREUnbox g d) (Tag2Type g) e IRTStar
 
-(* Γ⊑ ⊢ d ⊑ e : g ⊑ ★
+(* Γ⊑ ⊢ d ⊑ e : t ⊑ ★ , t ⊑ g
    ----------------------------------
-   Γ⊑ ⊢ d ⊑ unbox[g](d) : g ⊑ g	*)
-| PUnboxR : forall Γ d e g,
-    Precision Γ d (Tag2Type g) e IRTStar ->
-    Precision Γ d (Tag2Type g) (IREUnbox g e) (Tag2Type g)
+   Γ⊑ ⊢ d ⊑ unbox[g](d) : t ⊑ g	*)
+| PUnboxR : forall Γ d e t g,
+    t <| (Tag2Type g) ->
+    Precision Γ d t e IRTStar ->
+    Precision Γ d t (IREUnbox g e) (Tag2Type g)
 
 .
 
 
-Lemma PPT : forall Γ e1 t1 e2 t2, Precision Γ e1 t1 e2 t2 -> t1 <| t2.
+(* Γ⊑ ⊢ d ⊑ e : g ⊑ g
+   ----------------------------------
+   Γ⊑ ⊢ box[g](d) ⊑ box[g](e) : ★ ⊑ ★	*)
+Lemma BoxCongruent : forall Γ d e g,
+    Precision Γ d (Tag2Type g) e (Tag2Type g) ->
+    Precision Γ (IREBox g d) IRTStar (IREBox g e) IRTStar.
+Proof. eauto using Precision. Qed.
+
+(* Γ⊑ ⊢ d ⊑ e : ★ ⊑ ★
+   ----------------------------------
+   Γ⊑ ⊢ unbox[g](d) ⊑ unbox[g](e) : g ⊑ g	*)
+Lemma UnboxCongruent: forall Γ d e g,
+    Precision Γ d IRTStar e IRTStar ->
+    Precision Γ (IREUnbox g d) (Tag2Type g) (IREUnbox g e) (Tag2Type g).
+Proof. eauto using Precision, TPrecisionRefl. Qed.
+
+
+Lemma PPT : forall Γ e1 t1 e2 t2,
+    PEnvP Γ -> Precision Γ e1 t1 e2 t2 -> t1 <| t2.
 Proof.
-  intros Γ e1 t1 e2 t2 HP.
-  induction HP; auto using TPrecision, TPrecisionRefl.
-  - inversion IHHP1; subst; trivial.
+  unfold PEnvP.
+  intros Γ e1 t1 e2 t2 HPE HP.
+  induction HP; eauto using TPrecision, TPrecisionRefl.
+  - apply PRFun. trivial.
+    apply IHHP; intros.
+    inversion H0.
+    breakStrDec; eauto.
+    injection H2; intros; subst; trivial.
+  - apply IHHP1 in HPE. inversion HPE; trivial.
 Qed.
 
 
@@ -309,7 +295,7 @@ Lemma PrecisionType: forall Γ e t,
 Proof.
   intros Γ e t.
   split; intros H.
-  - induction H; eauto using Precision, InP12.
+  - induction H; eauto using Precision, InP12, TPrecisionRefl.
   - apply PrecisionType1 in H.
     rewrite Env2Env in H. trivial.
 Qed.
@@ -351,25 +337,103 @@ Qed.
 
 
 Ltac EnvUnique :=
-  match goal with 
+  match goal with
   [ H1: In ?Γ ?var = _,
     H2: In ?Γ ?var = _ |- _ ] =>
     rewrite H1 in H2; injection H2; intros; subst
   end.
 
+
+Definition EnvTrans (Γ1 Γ2 : PEnvironment) : Prop := PEnv2 Γ1 = PEnv1 Γ2.
+
+
+Fixpoint EnvJoin (Γ1 Γ2 : PEnvironment) : PEnvironment :=
+  match Γ1, Γ2 with
+  | MEmpty, MEmpty => MEmpty
+  | (MCons var (t1, _) Γ1'), (MCons _ (_, t3) Γ2') =>
+       MCons var (t1, t3) (EnvJoin Γ1' Γ2')
+  | _, _ => MEmpty
+  end.
+
+
+Lemma aux1 : forall var t1 t2 Γ1 Γ2,
+  EnvTrans (var |=> (t1, t2); Γ1) Γ2 ->
+  exists t3 Γ2', Γ2 = MCons var (t2, t3) Γ2' /\ EnvTrans Γ1 Γ2'.
+Proof.
+  unfold EnvTrans.
+  intros.
+  destruct Γ2.
+  - discriminate.
+  - destruct p. exists i0. exists Γ2.
+    simpl in H. injection H; intros; subst; intuition.
+Qed.
+
+
+Lemma aux2 : forall var t2 t3 Γ1 Γ2,
+  EnvTrans Γ1 (var |=> (t2, t3); Γ2) ->
+  exists t1 Γ1', Γ1 = MCons var (t1, t2) Γ1' /\ EnvTrans Γ1' Γ2.
+Proof.
+  unfold EnvTrans.
+  intros.
+  destruct Γ1.
+  - discriminate.
+  - destruct p. exists i. exists Γ1.
+    simpl in H. injection H; intros; subst; intuition.
+Qed.
+
+
+Lemma JoinE1 : forall Γ1 Γ2,
+    EnvTrans Γ1 Γ2 -> PEnv1 (EnvJoin Γ1 Γ2) = PEnv1 Γ1.
+Proof.
+  intros Γ1.
+  unfold EnvTrans.
+  induction Γ1; intros Γ2 H.
+  - simpl in H. destruct Γ2; easy.
+  - destruct a.
+    apply aux1 in H. destruct H as [? [? [? ?]]].
+    rewrite H. simpl.
+    f_equal. auto.
+Qed.
+
+
+Lemma JoinE2 : forall Γ1 Γ2,
+    EnvTrans Γ1 Γ2 -> PEnv2 (EnvJoin Γ1 Γ2) = PEnv2 Γ2.
+Proof.
+  unfold EnvTrans.
+  intros Γ1 Γ2.
+  generalize dependent Γ1.
+  induction Γ2; intros Γ1 H.
+  -  simpl in H. destruct Γ1; trivial.
+     destruct p. simpl in H. discriminate.
+  - destruct a.
+    apply aux2 in H. destruct H as [? [? [? ?]]].
+    rewrite H. simpl.
+    f_equal. auto.
+Qed.
+
+
+Lemma JoinTrans : forall Γ1 Γ2,
+  EnvTrans Γ1 Γ2 -> PEnvP Γ1 -> PEnvP Γ2 -> PEnvP (EnvJoin Γ1 Γ2).
+Proof.
+  intros Γ1 Γ2 HT HP1 HP2.
+  unfold PEnvP. intros.
+Abort.
+
 (*
-Lemma PrecisionTrans : forall Γ e1 t1 e2 t2 e3 t3,
-  Precision Γ e1 t1 e2 t2 ->
-  Precision Γ e2 t2 e3 t3 ->
-  Precision Γ e1 t1 e3 t3.
+Lemma PrecisionTrans : forall Γ12 Γ23 e1 t1 e2 t2 e3 t3,
+  EnvTrans Γ12 Γ23 -> PEnvP Γ12 -> PEnvP Γ23 ->
+  Precision Γ12 e1 t1 e2 t2 ->
+  Precision Γ23 e2 t2 e3 t3 ->
+  Precision (EnvJoin Γ12 Γ23) e1 t1 e3 t3.
 Proof with eauto using Precision.
-  intros Γ e1 t1 e2 t2 e3 t3 H12 H23.
+  intros Γ12 Γ23 e1 t1 e2 t2 e3 t3 HT HP12 HP23 H12 H23.
   generalize dependent e3.
   generalize dependent t3.
-  induction H12; intros ? ? H23; try easy.
+  generalize dependent Γ23.
+  induction H12; intros ? HT HP23 ? ? H23.
   - (* var *) inversion H23; subst.
-    + EnvUnique...
-    + inversion H0; subst. 
+    + eauto using Precision.
+    + inversion H0; subst.
       EnvUnique...
       NoTag2Star.
   - (* plus *) inversion H23; subst...
@@ -379,13 +443,13 @@ Proof with eauto using Precision.
     NoTag2Star.
   - (* set *) inversion H23; subst...
     NoTag2Star.
-  - (* fun *) inversion H23; subst; shelve. 
+  - (* fun *) inversion H23; subst; shelve.
   - (* funapp *) inversion H23; subst.
     + eapply PFunApp.
       apply IHPrecision1.
 
   inversion H23; subst;
-  try match goal with 
+  try match goal with
   [ H1: In ?Γ ?var = _,
     H2: In ?Γ ?var = _ |- _ ] => idtac H1 H2;
     rewrite H1 in H2; injection H2; intros; subst
@@ -396,7 +460,7 @@ Proof with eauto using Precision.
        eapply PUnboxL. eapply IHPrecision.
        inversion H2; subst.
        + NoTag2Star.
-       + 
+       +
   - apply PrecisionType1 in H23. inversion H23; subst.
     erewrite (InP1 _ var t1 (Tag2Type g)) in H3; trivial;
     inversion H3; subst; eauto using Precision.
@@ -408,7 +472,7 @@ Proof with eauto using Precision.
     eapply PBoxR.
 
   - apply Tag2TypeInjective in H; subst.
-    eapply PBoxR.    
+    eapply PBoxR.
     inversion H2; subst; eauto using Precision;
     NoTag2Star.
   - eapply PUnboxL.
@@ -419,13 +483,26 @@ Qed.
 Fixpoint Env2Dyn (Γ : IREnvironment) : PEnvironment :=
   match Γ with
   | MEmpty => MEmpty
-  | MCons k t Γ' => MCons k (pent t IRTStar (TPStar t)) (Env2Dyn Γ')
+  | MCons k t Γ' => MCons k (t,  IRTStar) (Env2Dyn Γ')
   end.
+
+
+Lemma EnvDynP : forall Γ, PEnvP (Env2Dyn Γ).
+Proof.
+  unfold PEnvP.
+  intros.
+  induction Γ.
+  - discriminate.
+  - simpl in *.
+    breakStrDec; auto.
+    injection H; intros; subst; auto using TPrecision.
+Qed.
+
 
 
 Lemma InEnv2Dyn : forall Γ var t,
   In Γ var = Some t ->
-  In (Env2Dyn Γ) var = Some (pent t IRTStar (TPStar t)).
+  In (Env2Dyn Γ) var = Some (t,  IRTStar).
 Proof.
   intros Γ var t H.
   induction Γ.
@@ -438,36 +515,14 @@ Qed.
 
 Lemma PrecisionDyn : forall Γ e t,
   Γ |= e : t -> Precision (Env2Dyn Γ) e t (dyn e) IRTStar.
-Proof.
+Proof with apply PUnboxR; eauto using TPrecision, TPrecisionRefl.
   intros Γ e t H.
-  induction H; simpl.
-  - replace IRTNil with (Tag2Type TgNil) by trivial.
-    eauto using Precision.
-  - eauto using Precision, InEnv2Dyn.
-  - replace IRTInt with (Tag2Type TgInt) by trivial.
-    eauto using Precision.
-  - replace IRTInt with (Tag2Type TgInt) by trivial.
-    apply PBoxR.
-    apply PPlus;
-    replace IRTInt with (Tag2Type TgInt) by trivial.
-    + apply PUnboxR. trivial.
-    + apply PUnboxR. trivial.
-  - replace IRTTbl with (Tag2Type TgTbl) by trivial.
-    eauto using Precision.
-  - replace IRTTbl with (Tag2Type TgTbl) by trivial.
-    eauto using Precision.
-  - apply PGet; trivial.
-    replace IRTTbl with (Tag2Type TgTbl) by trivial.
-    apply PUnboxR. trivial.
-  - apply PSet; trivial.
-    replace IRTTbl with (Tag2Type TgTbl) by trivial.
-    apply PUnboxR. trivial.
-  - assert (Precision (Env2Dyn Γ) (IREFun var t body) (IRTFun t t')
-                                  (IREFun var IRTStar (dyn body))
-                                     (IRTFun IRTStar IRTStar)).
-    { eauto using Precision. }
-      
-    
-    
+  induction H; simpl; eauto using Precision, TPrecision, InEnv2Dyn.
+  - apply PBoxR.
+    apply PPlus...
+  - apply PGet; trivial...
+  - apply PSet; trivial...
+  - eapply PFunApp; eauto...
+Qed.
 
 
